\documentclass{amsart}
\usepackage{amsfonts,amsmath,amssymb,amsthm}

\begin{document}
\section{Introduction}
{
    We prove some polynomial identities for determinants. 

    $\alpha,\beta,\gamma,\delta,\epsilon,\zeta,\eta,\theta,\iota,\kappa,\lambda,\zeta,\eta,\xi$ $o$ $\pi,\rho,\sigma,\tau,\upsilon,\phi,\chi,\psi,\omega$

    Steps are the following. 
    \begin{itemize}
        \item For $1\leq \zeta\leq \alpha$, expand $\det\begin{bmatrix}
            i_1&\cdots&i_\alpha&i_\zeta&r_1&\cdots&r_\beta\\
            j_1&\cdots&j_\alpha&j_{\alpha+1}&c_1&\cdots&c_\beta
        \end{bmatrix}$ along row $i_\zeta$. 

        \item For $1\leq\eta\leq\alpha+1$, expand $\det\begin{bmatrix}
            i_1&\cdots&i_\alpha&i_{\alpha+1}&r_1&\cdots&r_\beta\\
            j_1&\cdots&j_\alpha&j_{\alpha+1}&\cdots&j_\eta&\cdots
        \end{bmatrix}$ along column $j_\eta$, where $j_\eta$ replaces $c_\lambda$ for some $1\leq\lambda\leq\beta$. 

        \item Expand $\det\begin{bmatrix}
            i_1&\cdots&i_\alpha&i_{\alpha+1}&r_1&\cdots&r_\beta\\
            j_1&\cdots&j_\alpha&j_{\alpha+1}&c_1&\cdots&c_\beta
        \end{bmatrix}$ along row $i_{\alpha+1}$ and expand it along column $c_\lambda$ for some $1\leq \lambda\leq \beta$. 
    \end{itemize}
}

\section{Relative determinant}
{
}

\section{Induction formula}
{
    \subsection{step 1}
    {
        We have equations for $\zeta=1,\cdots,\alpha$ 
        \begin{align}
            0={}&(-1)^\alpha\sum_{\eta=1}^\alpha(-1)^{\eta-1}a^{i_\zeta}_{j_\eta}\det\begin{bmatrix}
                i_1\;\cdots&i_\alpha&r_1\;\cdots\; r_\beta\\
                \cdots\widehat{j_\eta}\cdots&j_{\alpha+1}&c_1\;\cdots\; c_\beta
            \end{bmatrix}\\
            &+a^{i_\zeta}_{j_{\alpha+1}}\det\begin{bmatrix}
                i_1\;\cdots\;i_\alpha&r_1\;\cdots\;r_\beta\\
                j_1\;\cdots\;j_\alpha&c_1\;\cdots\;c_\beta
            \end{bmatrix}\\
            &+\sum_{\lambda=1}^\beta(-1)^\lambda a^{i_\zeta}_{c_\lambda}\det\begin{bmatrix}
                i_1\;\cdots\;i_\alpha&r_1&\cdots\;r_\beta\\
                j_1\;\cdots\;j_\alpha&j_{\alpha+1}&\cdots\widehat{c_\lambda}\cdots
            \end{bmatrix}
        \end{align}
        We can solve such that for $\eta=1,\cdots,\alpha$
        \begin{align}
            &\det\begin{bmatrix}
                i_1\;\cdots&i_\alpha&r_1\;\cdots\;r_\beta\\
                \cdots\widehat{j_\eta}\cdots&j_{\alpha+1}&c_1\;\cdots\;c_\beta
            \end{bmatrix}\\
            ={}&\frac{1}{\det\begin{bmatrix}
                i_1\;\cdots\;i_\alpha\\
                j_1\;\cdots\;j_\alpha
            \end{bmatrix}}\Bigg(\det\begin{bmatrix}
                i_1\;\cdots&i_\alpha\\
                \cdots\widehat{j_\eta}\cdots&j_{\alpha+1}
            \end{bmatrix}\det\begin{bmatrix}
                i_1\;\cdots\;i_\alpha&r_1\;\cdots\;r_\beta\\
                j_1\;\cdots\;j_\alpha&c_1\;\cdots\;c_\beta
            \end{bmatrix}\\
            &\hspace{3eM}+\sum_{\lambda=1}^\beta(-1)^\lambda\det\begin{bmatrix}
                i_1\;\cdots&i_\alpha\\
                \cdots\widehat{j_\eta}\cdots&c_\lambda
            \end{bmatrix}\det\begin{bmatrix}
                i_1\;\cdots\;i_\alpha&r_1&\cdots\;r_\beta\\
                j_1\;\cdots\;j_\alpha&j_{\alpha+1}&\cdots\widehat{c_\lambda}\cdots
            \end{bmatrix}\Bigg)
        \end{align}
    }

    \subsection{step 2}
    {
        We have equations for $\eta=1,\cdots,\alpha+1$ 
        \begin{align}
            0&=\sum_{\zeta=1}^{\alpha+1}(-1)^{\lambda+\alpha+\zeta+1}a^{i_\zeta}_{j_\eta}\det\begin{bmatrix}
                \cdots\widehat{i_\zeta}\cdots&r_1&\cdots\;r_\beta\\
                j_1\;\cdots&j_{\alpha+1}&\cdots\widehat{c_\lambda}\cdots
            \end{bmatrix}\\
            &+\sum_{\kappa=1}^\beta(-1)^{\kappa+\lambda}a^{r_\kappa}_{j_\eta}\det\begin{bmatrix}
                i_1\;\cdots\;i_{\alpha+1}&\cdots\widehat{r_\kappa}\cdots\\
                j_1\;\cdots\;j_{\alpha+1}&\cdots\widehat{c_\lambda}\cdots
            \end{bmatrix}. 
        \end{align}
        We can solve such that for $\zeta=1,\cdots,\alpha+1$ 
        \begin{align}
            &\det\begin{bmatrix}
                \cdots\widehat{i_\zeta}\cdots&r_1&\cdots\;r_\beta\\
                j_1\;\cdots&j_{\alpha+1}&\cdots\widehat{c_\lambda}\cdots
            \end{bmatrix}\\
            ={}&\frac{1}{\det\begin{bmatrix}
                i_1\;\cdots\;i_{\alpha+1}\\
                j_1\;\cdots\;j_{\alpha+1}
            \end{bmatrix}}\sum_{\kappa=1}^\beta(-1)^{\kappa+1}\det\begin{bmatrix}
                \cdots\widehat{i_\zeta}\cdots&r_\kappa\\
                j_1\;\cdots&j_{\alpha+1}
            \end{bmatrix}\det\begin{bmatrix}
                i_1\;\cdots\;i_{\alpha+1}&\cdots\widehat{r_\kappa}\cdots\\
                j_1\;\cdots\;j_{\alpha+1}&\cdots\widehat{c_\lambda}\cdots
            \end{bmatrix}
        \end{align}
    }

    \subsection{step 3}
    {
        We finally have 
        \begin{align}
            &\det\begin{bmatrix}
                i_1\;\cdots\;i_\alpha&r_1\;\cdots\;r_\beta\\
                j_1\;\cdots\;j_\alpha&c_1\;\cdots\;c_\beta
            \end{bmatrix}\\
            ={}&\frac{1}{\det\begin{bmatrix}
                i_1\;\cdots\;i_{\alpha+1}\\
                j_1\;\cdots\;j_{\alpha+1}
            \end{bmatrix}}\sum_{\kappa,\lambda=1}^\beta(-1)^{\kappa+\lambda}\det\begin{bmatrix}
                i_1\;\cdots\;i_\alpha&r_\kappa\\
                j_1\;\cdots\;j_\alpha&c_\lambda
            \end{bmatrix}\det\begin{bmatrix}
                i_1\;\cdots\;i_{\alpha+1}&\cdots\widehat{r_\kappa}\cdots\\
                j_1\;\cdots\;j_{\alpha+1}&\cdots\widehat{c_\lambda}\cdots
            \end{bmatrix}\\
            &-(\beta-1)\frac{\det\begin{bmatrix}
                i_1\;\cdots\;i_\alpha\\
                j_1\;\cdots\;j_\alpha
            \end{bmatrix}}{\det\begin{bmatrix}
                i_1\;\cdots\;i_{\alpha+1}\\
                j_1\;\cdots\;j_{\alpha+1}
            \end{bmatrix}^2}\sum_{\kappa=1}^\beta(-1)^{\kappa+\lambda}\det\begin{bmatrix}
                i_1\;\cdots\;i_{\alpha+1}&r_\kappa\\
                j_1\;\cdots\;j_{\alpha+1}&c_\lambda
            \end{bmatrix}\det\begin{bmatrix}
                i_1\;\cdots\;i_{\alpha+1}&\cdots\widehat{r_\kappa}\cdots\\
                j_1\;\cdots\;j_{\alpha+1}&\cdots\widehat{c_\lambda}\cdots
            \end{bmatrix}
        \end{align}
        where the free index $\lambda$ can be $1,\cdots,\beta$. For rows $x_1,\cdots,x_n$ and rows $y_1,\cdots,y_n$, denote 
        \begin{align}
            \widetilde{\det}_\alpha\begin{bmatrix}
                x_1\;\cdots\;x_n\\y_1\;\cdots\;y_n
            \end{bmatrix}:=\frac{\det\begin{bmatrix}
                i_1\;\cdots\;i_\alpha&x_1\;\cdots\;x_n\\
                j_1\;\cdots\;j_\alpha&y_1\;\cdots\;y_n
            \end{bmatrix}}{\det\begin{bmatrix}
                i_1\;\cdots\;i_\alpha\\
                j_1\;\cdots\;j_\alpha
            \end{bmatrix}}. 
        \end{align}
        Then the above equation is 
        \begin{align}
            \widetilde{\det}_\alpha\begin{bmatrix}
                r_1\;\cdots\;r_\beta\\
                c_1\;\cdots\;c_\beta
            \end{bmatrix}={}&\sum_{\kappa,\lambda=1}^\beta(-1)^{\kappa+\lambda}\widetilde{\det}_\alpha\begin{bmatrix}
                r_\kappa\\
                c_\lambda
            \end{bmatrix}\widetilde{\det}_{\alpha+1}\begin{bmatrix}
                \cdots\widehat{r_\kappa}\cdots\\
                \cdots\widehat{c_\lambda}\cdots
            \end{bmatrix}\\
            &-(\beta-1)\sum_{\kappa=1}^\beta(-1)^{\kappa+\lambda}\widetilde{\det}_{\alpha+1}\begin{bmatrix}
                r_\kappa\\
                c_\lambda
            \end{bmatrix}\widetilde{\det}_{\alpha+1}\begin{bmatrix}
                \cdots\widehat{r_\kappa}\cdots\\
                \cdots\widehat{c_\lambda}\cdots
            \end{bmatrix}. 
        \end{align}

        \begin{proof}
            For rows $x_1,\cdots,x_n$ and rows $y_1,\cdots,y_n$, denote 
            \begin{align}
                \widetilde{\det}_\alpha\begin{bmatrix}
                    x_1\;\cdots\;x_n\\y_1\;\cdots\;y_n
                \end{bmatrix}:=\frac{\det\begin{bmatrix}
                    i_1\;\cdots\;i_\alpha&x_1\;\cdots\;x_n\\
                    j_1\;\cdots\;j_\alpha&y_1\;\cdots\;y_n
                \end{bmatrix}}{\det\begin{bmatrix}
                    i_1\;\cdots\;i_\alpha\\
                    j_1\;\cdots\;j_\alpha
                \end{bmatrix}}. 
            \end{align}
            Then $\widetilde{\det}_\alpha$ and $\det$ satisfy similar polynomial equations. In particular we expand $\widetilde{\det}_\alpha\begin{bmatrix}
                i_{\alpha+1}&r_1\;\cdots\;r_\beta\\
                j_{\alpha+1}&c_1\;\cdots\;c_\beta
            \end{bmatrix}$ along row $r_\kappa$ for $\kappa=1,\cdots,\beta$ and along column $j_{\alpha+1}$. We have 
            \begin{align}
                \widetilde{\det}_\alpha\begin{bmatrix}
                    i_{\alpha+1}&r_1\;\cdots\;r_\beta\\
                    j_{\alpha+1}&c_1\;\cdots\;c_\beta
                \end{bmatrix}={}& (-1)^\kappa\widetilde{\det}_\alpha\begin{bmatrix}
                    r_\kappa\\
                    j_{\alpha+1}
                \end{bmatrix}\widetilde{\det}_\alpha\begin{bmatrix}
                    i_{\alpha+1}&\cdots\;\widehat{r_\kappa}\;\cdots\\
                    c_1&\cdots\;c_\beta
                \end{bmatrix}\\
                &+\sum_{\lambda=1}^\beta(-1)^{\kappa+\lambda}\widetilde{\det}_\alpha\begin{bmatrix}
                    r_\kappa\\
                    c_\lambda
                \end{bmatrix}\widetilde{\det}_\alpha\begin{bmatrix}
                    i_{\alpha+1}&\cdots\;\widehat{r_\kappa}\;\cdots\\
                    j_{\alpha+1}&\cdots\;\widetilde{c_\lambda}\;\cdots
                \end{bmatrix}
            \end{align}
            and 
            \begin{align}
                \widetilde{\det}_\alpha\begin{bmatrix}
                    i_{\alpha+1}&r_1\;\cdots\;r_\beta\\
                    j_{\alpha+1}&c_1\;\cdots\;c_\beta
                \end{bmatrix}={}& \widetilde{\det}_\alpha\begin{bmatrix}
                    i_{\alpha+1}\\
                    j_{\alpha+1}
                \end{bmatrix}\widetilde{\det}_\alpha\begin{bmatrix}
                    r_1\;\cdots\;r_\beta\\
                    c_1\;\cdots\;c_\beta
                \end{bmatrix}\\
                &+\sum_{\kappa=1}^\beta(-1)^\kappa\widetilde{\det}_\alpha\begin{bmatrix}
                    r_\kappa\\
                    j_{\alpha+1}
                \end{bmatrix}\widetilde{\det}_\alpha\begin{bmatrix}
                    i_{\alpha+1}&\cdots\;\widehat{r_\kappa}\;\cdots\\
                    c_1&\cdots\;c_\beta
                \end{bmatrix}. 
            \end{align}
            We then have 
            \begin{align}
                \widetilde{\det}_\alpha\begin{bmatrix}
                    i_{\alpha+1}\\
                    j_{\alpha+1}
                \end{bmatrix}\widetilde{\det}_\alpha\begin{bmatrix}
                    r_1\;\cdots\;r_\beta\\
                    c_1\;\cdots\;c_\beta
                \end{bmatrix}={}&(-1)^\kappa\widetilde{\det}_\alpha\begin{bmatrix}
                    r_\kappa\\
                    j_{\alpha+1}
                \end{bmatrix}\widetilde{\det}_\alpha\begin{bmatrix}
                    i_{\alpha+1}&\cdots\;\widehat{r_\kappa}\;\cdots\\
                    c_1&\cdots\;c_\beta
                \end{bmatrix}\\
                &+\sum_{\lambda=1}^\beta(-1)^{\kappa+\lambda}\widetilde{\det}_\alpha\begin{bmatrix}
                    r_\kappa\\
                    c_\lambda
                \end{bmatrix}\widetilde{\det}_\alpha\begin{bmatrix}
                    i_{\alpha+1}&\cdots\;\widehat{r_\kappa}\;\cdots\\
                    j_{\alpha+1}&\cdots\;\widehat{c_\lambda}\;\cdots
                \end{bmatrix}\\
                &-\sum_{\kappa=1}^\beta(-1)^\kappa\widetilde{\det}_\alpha\begin{bmatrix}
                    r_\kappa\\
                    j_{\alpha+1}
                \end{bmatrix}\widetilde{\det}_\alpha\begin{bmatrix}
                    i_{\alpha+1}&\cdots\;\widehat{r_\kappa}\;\cdots\\
                    c_1&\cdots\;c_\beta
                \end{bmatrix}.
            \end{align}
        \end{proof}
    }
}

\appendix
\section{Induction formula}
{
    Consider the function $\delta_\kappa:\{1,\cdots,\beta-1\}\to\{1,\cdots,\beta\}$ skipping $\kappa$ for $1\leq \kappa\leq\beta$. Let $F(\kappa_1,\kappa_2)$ be a function of two variables. Denote 
    \begin{align*}
        \mathrm{ord}(\kappa_1,\kappa_2):=\begin{cases}
            1,&\kappa_1<\kappa_2\\
            -1,&\kappa_1>\kappa_2. 
        \end{cases}
    \end{align*}
    We have 
    \begin{align*}
        \sum_{\kappa=1}^\beta\sum_{\kappa'=1}^{\beta-1}(-1)^{\kappa+\kappa'}F(\kappa,\delta_\kappa(\kappa'))=-\sum_{\kappa_1\ne\kappa_2}(-1)^{\kappa_1+\kappa_2}\mathrm{ord}(\kappa_1,\kappa_2)F(\kappa_1,\kappa_2)
    \end{align*}

    \begin{align*}
        &\sum_{\kappa_1=1}^\beta\sum_{\kappa_2=1}^{\beta-1}\sum_{\kappa_3=1}^{\beta-2}(-1)^{\kappa_1+\kappa_2+\kappa_3}F\big(\kappa_1,\delta_{\kappa_1}(\kappa_2),\delta_{\kappa_1}\delta_{\kappa_2}(\kappa_3)\big)\\
        =&-\sum_{1\leq k_1<k_2<k_3\leq \beta}(-1)^{k(1)+k(2)+k(3)}\sum_{\sigma\in S_3}\mathrm{sgn}(\sigma)F\big(k(\sigma(1)),k(\sigma(2)),k(\sigma(3))\big)
    \end{align*}

    \begin{align*}
        &\sum_{\kappa_1=1}^\beta\sum_{\kappa_2=1}^{\beta-1}\cdots\sum_{\kappa_m=1}^{\beta-m+1}(-1)^{\kappa_1+\cdots+\kappa_m}F\Big(\kappa_1,\delta_{\kappa_1}(\kappa_2),\cdots,\delta_{\kappa_1}\delta_{\kappa_2}\cdots\delta_{\kappa_{m-1}}(\kappa_m)\Big)\\
        ={}&(-1)^{\binom{m}{2}}\sum_{1\leq k_1<\cdots<k_m\leq \beta}(-1)^{k_1+\cdots+k_m}\sum_{\sigma\in S_m}\mathrm{sgn}(\sigma)F\Big(k_{\sigma(1)},\cdots,k_{\sigma(m)}\Big)
    \end{align*}

    Consider the case when $F(x_1,\cdots,x_m)$ has the form 
    \begin{align*}
        F(x_1,\cdots,x_m)=F_1(x_1)\cdots F_m(x_m) F_{\mathrm{sym}}(x_1,\cdots,x_m)
    \end{align*}
    where $F_{\mathrm{sym}}$ is symmetric with respect to $S_m$. The identity becomes 
    \begin{align*}
        &\sum_{\kappa_1=1}^\beta\sum_{\kappa_2=1}^{\beta-1}\cdots\sum_{\kappa_m=1}^{\beta-m+1}(-1)^{\kappa_1+\cdots+\kappa_m}F\Big(\kappa_1,\delta_{\kappa_1}(\kappa_2),\cdots,\delta_{\kappa_1}\delta_{\kappa_2}\cdots\delta_{\kappa_{m-1}}(\kappa_m)\Big)\\
        ={}&(-1)^{\binom{m}{2}}\sum_{1\leq k_1<\cdots<k_m\leq \beta}(-1)^{k_1+\cdots+k_m}\det\big(F_i(k_j)\big)F_{\mathrm{sym}}(k_1,\cdots,k_m). 
    \end{align*}
}
\end{document}
